rewriting_system.v
@@ -2,16 +2,56 @@ Require Import Relations.
 
 
 
-Module Type REWRITING_SYSTEM.
+Class REWRITING_SYSTEM :=
+{
+    configuration : Set;
+    transition    : configuration -> configuration -> Prop
+}.
 
-  Parameters
-  (configuration : Set)
-  (transition    : configuration -> configuration -> Prop).
 
-  Notation "c1 → c2"  := (transition c1 c2)              (no associativity, at level 70).
-  Notation "t1 →+ t2" := (clos_trans_1n _ transition t1 t2) 
+Notation "`( rw ) c1 → c2"  := (@transition rw c1 c2)
+                                         (no associativity, at level 70, c1 at level 69).
+Notation "`( rw ) c1 →+ c2" := (clos_trans_1n _ (@transition rw) c1 c2)
+                                         (no associativity, at level 70, c1 at level 69).
+Notation "`( rw ) c1 →* c2" := (clos_refl_trans_1n _ (@transition rw) c1 c2)
+                                         (no associativity, at level 70, c1 at level 69).
+
+Notation "c1 → c2"  := (transition c1 c2)                (no associativity, at level 70).
+Notation "c1 →+ c2" := (clos_trans_1n _ transition c1 c2)
                                                          (no associativity, at level 70).
-  Notation "t1 →* t2" := (clos_refl_trans_1n _ transition t1 t2) 
+Notation "c1 →* c2" := (clos_refl_trans_1n _ transition c1 c2)
                                                          (no associativity, at level 70).
 
-End REWRITING_SYSTEM.
+
+
+
+Class LABELED_REWRITING_SYSTEM :=
+{
+    label          : Set; 
+    lconfiguration : Set;
+    ltransition    : label -> lconfiguration -> lconfiguration -> Prop
+}.
+
+
+Notation "`( rw ) l |~ c1 → c2"  := (@ltransition rw l c1 c2)
+                                      (no associativity, at level 70, c1, l at level 69).
+Notation "`( rw ) l |~ c1 →+ c2" := (clos_trans_1n _ (@ltransition rw l) c1 c2)
+                                      (no associativity, at level 70, c1, l at level 69).
+Notation "`( rw ) l |~ c1 →* c2" := (clos_refl_trans_1n _ (@ltransition rw l) c1 c2)
+                                      (no associativity, at level 70, c1, l at level 69).
+
+Notation "l |~ c1 → c2"  := (ltransition l c1 c2)
+                                         (no associativity, at level 70, c1 at level 69).
+Notation "l |~ c1 →+ c2" := (clos_trans_1n _ (ltransition l) c1 c2)
+                                         (no associativity, at level 70, c1 at level 69).
+Notation "l |~ c1 →* c2" := (clos_refl_trans_1n _ (ltransition l) c1 c2)
+                                         (no associativity, at level 70, c1 at level 69).
+
+
+
+Instance LRWS_is_RWS (_ : REWRITING_SYSTEM) : LABELED_REWRITING_SYSTEM :=
+{
+    label          := unit;
+    lconfiguration := configuration;
+    ltransition    := fun (_ : unit) => transition
+}.
