reduction_semantics_facts.v
@@ -31,17 +31,15 @@ Module Type DET_RED_MINI_SEM.
       exists {k'} (c : context k k') (r : redex k') t,  dec t1 k (d_red r c) /\
           contract r = Some t /\ t2 = c[t].
 
-  Notation "k |~ t1 → t2"  := (reduce k t1 t2)   (no associativity, at level 70).
-  Notation "k |~ t1 →+ t2" := (clos_trans_1n _ (reduce k) t1 t2) 
-                                                  (no associativity, at level 70).
-  Notation "k |~ t1 →* t2" := (clos_refl_trans_1n _ (reduce k) t1 t2) 
-                                                  (no associativity, at level 70).
+  Notation "k |~ t1 → t2"  := (reduce k t1 t2) 
+                                         (no associativity, at level 70, t1 at level 69).
 
 
-  Axiom dec_is_pfunction : forall {t k} {d d0 : decomp k}, 
-                               dec t k d -> dec t k d0 -> d = d0.
+  Axiom dec_is_det : forall {t k} {d d0 : decomp k}, 
+                         dec t k d -> dec t k d0 -> d = d0.
 
 End DET_RED_MINI_SEM.
+
 
 
 
@@ -50,8 +48,23 @@ Module DET_RED_SEM_Facts (R : DET_RED_MINI_SEM).
   Module RF := RED_LANG_Facts R.
   Import R RF.
 
+
+  Lemma reduce_is_det :                                                forall t1 t2 t3 k,
+      k |~ t1 → t2  ->  k |~ t1 → t3  ->  t2 = t3.
+
+  Proof.
+    intros t1 t2 t3 k H H0.
+    destruct H  as [k2 [c1 [r1 [t1' [G  [G0 G1]]]]]],
+             H0 as [k3 [c2 [r2 [t2' [G2 [G3 G4]]]]]];
+    subst.
+    assert (H : d_red r1 c1 = d_red r2 c2) by eauto using dec_is_det.
+    inversion H; dep_subst.
+    congruence.
+ Qed.
+
+
   Lemma reduce_red : 
-      forall {k1 k2} (c : context k1 k2) (r : redex k2) t,  k1 |~ d_red r c → t  ->
+      forall {k1 k2} (c : context k1 k2) (r : redex k2) t,  k1 |~ c[r] → t  ->
           exists t', contract r = Some t' /\ t = c[t'].
 
   Proof.
@@ -60,7 +73,7 @@ Module DET_RED_SEM_Facts (R : DET_RED_MINI_SEM).
     destruct H as [k' [c' [r' [t' [H0 [H1 H2]]]]]].
     
     assert (H3 : d_red r c = d_red r' c'). 
-    { eapply dec_is_pfunction; solve [reflexivity | unfold dec; eauto]. }
+    { eapply dec_is_det; solve [reflexivity | unfold dec; eauto]. }
     inversion H3; dep_subst.
     eauto.
   Qed.
