rewriting_system_following.v
@@ -1,0 +1,36 @@
+Require Import Vector
+               rewriting_system.
+
+Import VectorNotations.
+Infix "++" := append.
+
+Fixpoint fin_lift1 {n} (m : Fin.t n) := match m with
+| Fin.F1 n   => @Fin.F1 (S n)
+| Fin.FS _ m => Fin.FS (fin_lift1 m)
+end.
+
+Coercion fin_lift1 : Fin.t >-> Fin.t.
+
+
+Class RW_FOLLOWING (Follower Followed : REWRITING_SYSTEM) :=
+{
+    semantics : (@configuration Follower) -> (@configuration Followed);
+
+    correct :                                                             forall cr1 cr2,
+        `(Follower) cr1 → cr2  ->  semantics cr1 = semantics cr2  \/  
+                                   `(Followed) semantics cr1 → semantics cr2;
+
+    complete :                                                        forall cd1 cd2 cr1,
+        `(Followed) cd1 → cd2  ->  semantics cr1 = cd1 -> 
+            exists n (crs : Vector.t configuration n) cr2,
+            (**)Forall (fun cr => semantics cr = cd1) crs /\
+            (**)semantics cr2 = cd2                       /\
+            (**)forall m : Fin.t (n+1), 
+                    (cr1 :: crs ++ [cr2])[@m] → (crs ++ [cr2])[@m];
+
+    no_silent_loops :
+      ~ exists crs : nat -> configuration, (*a stream of configurations*)
+          forall n, 
+          (**)  `(Follower) crs n  →  crs (S n)  /\ 
+          (**)~ `(Followed) semantics (crs n)  →  semantics (crs (S n))
+}.
